add spec for lanes a m = 2 and lanes a m = 16

code/sha2-vec/Hacl.Spec.SHA2.Lemmas.fst
@@ -12,6 +12,29 @@ open Hacl.Spec.SHA2.Vec
 
 #set-options "--z3rlimit 50 --fuel 0 --ifuel 1"
 
+val transpose_ws2_lemma_ij:
+    #a:sha2_alg
+  -> #m:m_spec{lanes a m == 2}
+  -> ws:ws_spec a m
+  -> j:nat{j < lanes a m}
+  -> i:nat{i < 16} ->
+  Lemma
+   (let l = lanes a m in
+    (vec_v (transpose_ws2 ws).[i]).[j] == (vec_v ws.[i / l * l + j]).[i % l])
+
+let transpose_ws2_lemma_ij #a #m ws j i =
+  let l = lanes a m in
+  let i_sub = i / l in
+  let j_sub = i % l in
+  assert (i_sub * l + j_sub == i);
+
+  let vs = sub ws (i_sub * l) l in
+  eq_intro (sub (transpose_ws2 ws) (i_sub * l) l) (transpose2x2_lseq vs);
+  assert ((vec_v (transpose_ws2 ws).[i]).[j] == (vec_v (transpose2x2_lseq vs).[j_sub]).[j]);
+  transpose2x2_lemma vs;
+  assert ((vec_v (transpose_ws2 ws).[i]).[j] == (vec_v ws.[i_sub * lanes a m + j]).[j_sub])
+
+
 val transpose_ws4_lemma_ij:
     #a:sha2_alg
   -> #m:m_spec{lanes a m == 4} // lanes a m * lanes a m = 16
@@ -61,6 +84,29 @@ let transpose_ws8_lemma_ij #a #m ws j i =
   assert ((vec_v (transpose_ws8 ws).[i]).[j] == (vec_v ws.[i_sub * lanes a m + j]).[j_sub])
 
 
+val transpose_ws16_lemma_ij:
+    #a:sha2_alg
+  -> #m:m_spec{lanes a m == 16}
+  -> ws:ws_spec a m
+  -> j:nat{j < lanes a m}
+  -> i:nat{i < 16} ->
+  Lemma
+   (let l = lanes a m in
+    (vec_v (transpose_ws16 ws).[i]).[j] == (vec_v ws.[i / l * l + j]).[i % l])
+
+let transpose_ws16_lemma_ij #a #m ws j i =
+  let l = lanes a m in
+  let i_sub = i / l in
+  let j_sub = i % l in
+  assert (i_sub * l + j_sub == i);
+
+  let vs = sub ws (i_sub * l) l in
+  //eq_intro (sub (transpose_ws16 ws) (i_sub * l) l) (transpose16x16_lseq vs);
+  assert ((vec_v (transpose_ws16 ws).[i]).[j] == (vec_v (transpose16x16_lseq vs).[j_sub]).[j]);
+  transpose16x16_lemma vs;
+  assert ((vec_v (transpose_ws16 ws).[i]).[j] == (vec_v ws.[i_sub * lanes a m + j]).[j_sub])
+
+
 val transpose_ws_lemma_ij:
     #a:sha2_alg
   -> #m:m_spec
@@ -75,9 +121,33 @@ let transpose_ws_lemma_ij #a #m ws j i =
   assert (((ws_spec_v (transpose_ws ws)).[j]).[i] == (vec_v (transpose_ws ws).[i]).[j]);
   match lanes a m with
   | 1 -> ()
+  | 2 -> transpose_ws2_lemma_ij #a #m ws j i
   | 4 -> transpose_ws4_lemma_ij #a #m ws j i
   | 8 -> transpose_ws8_lemma_ij #a #m ws j i
-  | _ -> admit()
+  | 16 -> transpose_ws16_lemma_ij #a #m ws j i
+
+
+val transpose_state2_lemma:
+    #a:sha2_alg
+  -> #m:m_spec{lanes a m == 2}
+  -> st:state_spec a m
+  -> j:nat{j < lanes a m}
+  -> i:nat{i < 8 * word_length a} ->
+  Lemma
+   (let l = lanes a m in
+    let ind = 8 * j + i / word_length a in
+    Seq.index (vec_v (transpose_state st).[ind / l]) (ind % l) ==
+    Seq.index (state_spec_v st).[j] (i / word_length a))
+
+let transpose_state2_lemma #a #m st j i =
+  let r0 = transpose2x2_lseq (sub st 0 2) in
+  transpose2x2_lemma (sub st 0 2);
+  let r1 = transpose2x2_lseq (sub st 2 2) in
+  transpose2x2_lemma (sub st 2 2);
+  let r3 = transpose2x2_lseq (sub st 4 2) in
+  transpose2x2_lemma (sub st 4 2);
+  let r4 = transpose2x2_lseq (sub st 6 2) in
+  transpose2x2_lemma (sub st 6 2)
 
 
 val transpose_state4_lemma:
@@ -118,6 +188,44 @@ let transpose_state8_lemma #a #m st j i =
   transpose8x8_lemma st
 
 
+val transpose_state16_lemma:
+    #a:sha2_alg
+  -> #m:m_spec{lanes a m == 16}
+  -> st:state_spec a m
+  -> j:nat{j < lanes a m}
+  -> i:nat{i < 8 * word_length a} ->
+  Lemma
+   (let l = lanes a m in
+    let ind = 8 * j + i / word_length a in
+    Seq.index (vec_v (transpose_state16 st).[ind / l]) (ind % l) ==
+    Seq.index (state_spec_v st).[j] (i / word_length a))
+
+let transpose_state16_lemma #a #m st j i =
+  let st16 = create 16 (zero_element a m) in
+  let st16 = update_sub st16 0 8 st in
+  let st_r = transpose16x16_lseq st16 in
+  transpose16x16_lemma st16;
+  assert (forall (i:nat{i < 8}) (j:nat{j < 8}). (vec_v st_r.[i]).[j] == (vec_v st.[j]).[i]);
+  let (st0,st1,st2,st3,st4,st5,st6,st7) = (st_r.[0],st_r.[1],st_r.[2],st_r.[3],st_r.[4],st_r.[5],st_r.[6],st_r.[7]) in
+  let (st8,st9,st10,st11,st12,st13,st14,st15) = (st_r.[8],st_r.[9],st_r.[10],st_r.[11],st_r.[12],st_r.[13],st_r.[14],st_r.[15]) in
+  let st0' = vec_interleave_low_n 8 st0 st1 in
+  vec_interleave_low_n_lemma_uint32_16_8 st0 st1;
+  let st1' = vec_interleave_low_n 8 st2 st3 in
+  vec_interleave_low_n_lemma_uint32_16_8 st2 st3;
+  let st2' = vec_interleave_low_n 8 st4 st5 in
+  vec_interleave_low_n_lemma_uint32_16_8 st4 st5;
+  let st3' = vec_interleave_low_n 8 st6 st7 in
+  vec_interleave_low_n_lemma_uint32_16_8 st6 st7;
+  let st4' = vec_interleave_low_n 8 st8 st9 in
+  vec_interleave_low_n_lemma_uint32_16_8 st8 st9;
+  let st5' = vec_interleave_low_n 8 st10 st11 in
+  vec_interleave_low_n_lemma_uint32_16_8 st10 st11;
+  let st6' = vec_interleave_low_n 8 st12 st13 in
+  vec_interleave_low_n_lemma_uint32_16_8 st12 st13;
+  let st7' = vec_interleave_low_n 8 st14 st15 in
+  vec_interleave_low_n_lemma_uint32_16_8 st14 st15
+
+
 val transpose_state_lemma_ij:
     #a:sha2_alg
   -> #m:m_spec
@@ -133,6 +241,7 @@ val transpose_state_lemma_ij:
 let transpose_state_lemma_ij #a #m st j i =
   match lanes a m with
   | 1 -> ()
+  | 2 -> transpose_state2_lemma #a #m st j i
   | 4 -> transpose_state4_lemma #a #m st j i
   | 8 -> transpose_state8_lemma #a #m st j i
-  | _ -> admit()
+  | 16 -> transpose_state16_lemma #a #m st j i
