lib/Lib.IntVector.Transpose.fsti
@@ -5,7 +5,10 @@ open Lib.IntTypes
 open Lib.Sequence
 open Lib.IntVector
 
-#set-options "--z3rlimit 50 --max_fuel 0 --max_ifuel 0"
+#set-options "--z3rlimit 50 --fuel 0 --ifuel 0"
+
+inline_for_extraction noextract
+let vec_t2 (t:v_inttype) = vec_t t 2 & vec_t t 2
 
 inline_for_extraction noextract
 let vec_t4 (t:v_inttype) = vec_t t 4 & vec_t t 4 & vec_t t 4 & vec_t t 4
@@ -18,29 +21,38 @@ let vec_t16 (t:v_inttype) = vec_t t 16 & vec_t t 16 & vec_t t 16 & vec_t t 16 & 
 
 
 inline_for_extraction noextract
-val transpose4x4: #t:v_inttype -> vec_t4 t -> vec_t4 t
+val transpose2x2: #t:v_inttype -> vec_t2 t -> vec_t2 t
 
 inline_for_extraction noextract
-val transpose8x8: #t:v_inttype -> vec_t8 t -> vec_t8 t
+val transpose4x4: #t:v_inttype{t = U32 \/ t = U64} -> vec_t4 t -> vec_t4 t
 
 inline_for_extraction noextract
-val transpose16x16: #t:v_inttype -> vec_t16 t & vec_t16 t -> vec_t16 t & vec_t16 t
+val transpose8x8: #t:v_inttype{t = U32 \/ t = U64} -> vec_t8 t -> vec_t8 t
+
+inline_for_extraction noextract
+val transpose16x16: #t:v_inttype{t = U32} -> vec_t16 t & vec_t16 t -> vec_t16 t & vec_t16 t
 
 
 inline_for_extraction noextract
-let transpose4x4_lseq (#t:v_inttype) (vs:lseq (vec_t t 4) 4) : lseq (vec_t t 4) 4 =
+let transpose2x2_lseq (#t:v_inttype) (vs:lseq (vec_t t 2) 2) : lseq (vec_t t 2) 2 =
+  let (v0,v1) = (vs.[0],vs.[1]) in
+  let (r0,r1) = transpose2x2 (v0,v1) in
+  create2 r0 r1
+
+inline_for_extraction noextract
+let transpose4x4_lseq (#t:v_inttype{t = U32 \/ t = U64}) (vs:lseq (vec_t t 4) 4) : lseq (vec_t t 4) 4 =
   let (v0,v1,v2,v3) = (vs.[0],vs.[1],vs.[2],vs.[3]) in
   let (r0,r1,r2,r3) = transpose4x4 (v0,v1,v2,v3) in
   create4 r0 r1 r2 r3
 
 inline_for_extraction noextract
-let transpose8x8_lseq (#t:v_inttype) (vs:lseq (vec_t t 8) 8) : lseq (vec_t t 8) 8 =
+let transpose8x8_lseq (#t:v_inttype{t = U32 \/ t = U64}) (vs:lseq (vec_t t 8) 8) : lseq (vec_t t 8) 8 =
   let (v0,v1,v2,v3,v4,v5,v6,v7) = (vs.[0],vs.[1],vs.[2],vs.[3],vs.[4],vs.[5],vs.[6],vs.[7]) in
   let (r0,r1,r2,r3,r4,r5,r6,r7) = transpose8x8 (v0,v1,v2,v3,v4,v5,v6,v7) in
   create8 r0 r1 r2 r3 r4 r5 r6 r7
 
 inline_for_extraction noextract
-let transpose16x16_lseq (#t:v_inttype) (vs:lseq (vec_t t 16) 16) : lseq (vec_t t 16) 16 =
+let transpose16x16_lseq (#t:v_inttype{t = U32}) (vs:lseq (vec_t t 16) 16) : lseq (vec_t t 16) 16 =
   let (v0,v1,v2,v3,v4,v5,v6,v7) = (vs.[0],vs.[1],vs.[2],vs.[3],vs.[4],vs.[5],vs.[6],vs.[7]) in
   let (v8,v9,v10,v11,v12,v13,v14,v15) = (vs.[8],vs.[9],vs.[10],vs.[11],vs.[12],vs.[13],vs.[14],vs.[15]) in
   let ((r0,r1,r2,r3,r4,r5,r6,r7),(r8,r9,r10,r11,r12,r13,r14,r15)) =
@@ -48,11 +60,14 @@ let transpose16x16_lseq (#t:v_inttype) (vs:lseq (vec_t t 16) 16) : lseq (vec_t t
   create16 r0 r1 r2 r3 r4 r5 r6 r7 r8 r9 r10 r11 r12 r13 r14 r15
 
 
-val transpose4x4_lemma: #t:v_inttype -> vs:lseq (vec_t t 4) 4 ->
+val transpose2x2_lemma: #t:v_inttype -> vs:lseq (vec_t t 2) 2 ->
+  Lemma (forall (i:nat{i < 2}) (j:nat{j < 2}). (vec_v (transpose2x2_lseq vs).[i]).[j] == (vec_v vs.[j]).[i])
+
+val transpose4x4_lemma: #t:v_inttype{t = U32 \/ t = U64} -> vs:lseq (vec_t t 4) 4 ->
   Lemma (forall (i:nat{i < 4}) (j:nat{j < 4}). (vec_v (transpose4x4_lseq vs).[i]).[j] == (vec_v vs.[j]).[i])
 
-val transpose8x8_lemma: #t:v_inttype -> vs:lseq (vec_t t 8) 8 ->
+val transpose8x8_lemma: #t:v_inttype{t = U32 \/ t = U64} -> vs:lseq (vec_t t 8) 8 ->
   Lemma (forall (i:nat{i < 8}) (j:nat{j < 8}). (vec_v (transpose8x8_lseq vs).[i]).[j] == (vec_v vs.[j]).[i])
 
-val transpose16x16_lemma: #t:v_inttype -> vs:lseq (vec_t t 16) 16 ->
+val transpose16x16_lemma: #t:v_inttype{t = U32} -> vs:lseq (vec_t t 16) 16 ->
   Lemma (forall (i:nat{i < 16}) (j:nat{j < 16}). (vec_v (transpose16x16_lseq vs).[i]).[j] == (vec_v vs.[j]).[i])
